Introduce the notion of "Frame Shift Assertions", and use to prove the rules about inv and auth at once for pvs and wp
Yeah, the name is horrible... but on the plus side, I think it should be possible to show that atomic triples and atomic shifts are also frame shift assertions, and then we get all this stuff for them for free.

program_logic/pviewshifts.v
@@ -179,3 +179,61 @@ Proof.
 Qed.
 
 End pvs.
+
+(** * Frame Shift Assertions. *)
+Section fsa.
+Context {Λ : language} {Σ : iFunctor} {A : Type}.
+Implicit Types P : iProp Λ Σ.
+Implicit Types Q : A → iProp Λ Σ.
+
+(* Yes, the name is horrible...
+   Frame Shift Assertions take a mask and a predicate over some type (that's
+   their "postcondition"). They support weakening the mask, framing resources
+   into the postcondition, and composition witn mask-changing view shifts. *)
+Class FrameShiftAssertion (FSA : coPset → (A → iProp Λ Σ) → iProp Λ Σ) := {
+  fsa_mask_frame_mono E1 E2 Q Q' :> E1 ⊆ E2 →
+                                 (∀ a, Q a ⊑ Q' a) → FSA E1 Q ⊑ FSA E2 Q';
+  fsa_trans3 E1 E2 Q : E2 ⊆ E1 →
+                     pvs E1 E2 (FSA E2 (λ a, pvs E2 E1 (Q a))) ⊑ FSA E1 Q;
+  fsa_frame_r E P Q : (FSA E Q ★ P) ⊑ FSA E (λ a, Q a ★ P)
+}.
+
+Context FSA `{FrameShiftAssertion FSA}.
+Lemma fsa_mono E Q Q' : (∀ a, Q a ⊑ Q' a) → FSA E Q ⊑ FSA E Q'.
+Proof. apply fsa_mask_frame_mono; auto. Qed.
+Lemma fsa_mask_weaken E1 E2 Q : E1 ⊆ E2 → FSA E1 Q ⊑ FSA E2 Q.
+Proof. intros. apply fsa_mask_frame_mono; auto. Qed.
+Lemma fsa_frame_l E P Q :
+  (P ★ FSA E Q) ⊑ FSA E (λ a, P ★ Q a).
+Proof.
+  rewrite commutative fsa_frame_r. apply fsa_mono=>a.
+  by rewrite commutative.
+Qed.
+Lemma fsa_strip_pvs E P Q : P ⊑ FSA E Q → pvs E E P ⊑ FSA E Q.
+Proof.
+  move=>->. rewrite -{2}fsa_trans3; last reflexivity.
+  apply pvs_mono, fsa_mono=>a. apply pvs_intro.  
+Qed.
+Lemma fsa_mono_pvs E Q Q' : (∀ a, Q a ⊑ pvs E E (Q' a)) → FSA E Q ⊑ FSA E Q'.
+Proof.
+  move=>HQ. rewrite -[FSA E Q']fsa_trans3; last reflexivity.
+  rewrite -pvs_intro. by apply fsa_mono.
+Qed.
+
+End fsa.
+
+(** View shifts are a FSA. *)
+Section pvs_fsa.
+Context {Λ : language} {Σ : iFunctor}.
+Implicit Types P : iProp Λ Σ.
+Implicit Types Q : () → iProp Λ Σ.
+
+Global Instance pvs_fsa : FrameShiftAssertion (λ E Q, pvs E E (Q ())).
+Proof.
+  split; intros.
+  - apply pvs_mask_frame_mono; auto.
+  - apply pvs_trans3; auto.
+  - apply pvs_frame_r; auto.
+Qed.
+
+End pvs_fsa.
